CKTInput.dfy
@@ -1,0 +1,79 @@
+include "objects.dfy"
+include "turing_machine.dfy"
+include "certificate.dfy"
+predicate isInputCKT (input:seq<string>)
+{
+    forall pos:nat::pos<|input| ==> isInputCKT'(input,pos)
+}
+predicate isStringAGate(str:string)
+{
+    str=="AND" || str=="OR" || str=="NOR"
+}
+predicate isAGoodPozInput(nr:string,poz:nat)
+    requires isStringAValidNumber(nr)
+{
+    poz-1-stringToNat(nr)>=0
+}
+predicate isAGoodVariableInput(x:string)
+{
+    !(x in ReservedWords) && !isStringAValidNumber(x)
+}
+predicate isStringAValidPos(input:seq<string>, pos:nat)
+    requires pos<|input|
+    requires isStringAValidNumber(input[pos])
+{
+    pos-1-stringToNat(input[pos])>=0 && !isStringAValidNumber(input[pos-1-stringToNat(input[pos])])
+}
+predicate isInputCKT' (input:seq<string>, pos:nat)
+    requires pos<|input|
+{
+    match input[pos]
+        case "AND" => 2<pos<|input| && isStringAValidNumber(input[pos-1]) && isStringAValidPos(input, pos-1) && isStringAValidNumber(input[pos-2]) && isStringAValidPos(input, pos-2)
+        case "OR" => 2<pos<|input| && isStringAValidNumber(input[pos-1]) && isStringAValidPos(input, pos-1) && isStringAValidNumber(input[pos-2]) && isStringAValidPos(input, pos-2)
+        case "NOT" => 1<pos<|input|&& isStringAValidNumber(input[pos-1]) && isStringAValidPos(input, pos-1) 
+        case x => if isStringAValidNumber(x) then isStringAValidPos(input, pos)
+                    else !(x in ReservedWords)
+}
+
+ lemma Lemma_ValidInputExtension(input: seq<string>, ext: seq<string>)
+    requires isInputCKT(input)
+    requires forall k :: |input| <= k <|input|+ |ext| ==> isInputCKT'(input + ext, k)
+    ensures isInputCKT(input + ext)
+{
+    var combined := input+ ext;
+    assert forall i :: 0 <= i < |input| ==> combined[i] == input[i];
+    assert forall i :: 0 <= i < |input| ==> isInputCKT'(input, i);
+    assert forall i :: 0 <= i < |input| && isInputCKT'(input,i)==> isInputCKT'(combined, i);
+}
+predicate isCertificateValidForInput (input:seq<string>,k:seq<string>)
+    requires isCertificateCorrectForm(k)
+{
+    forall pos:nat:: pos<|input| ==> if !(input[pos] in ReservedWords) && !isStringAValidNumber(input[pos]) then (input[pos] in k) else true
+}
+ghost predicate isLanguageCKT(l:Language)
+{
+    forall input:seq<string> :: (input in l) <==> exists pos:nat:: 1<=pos<|input|-3 
+                                            && isInputCKT(input) 
+}
+ghost predicate isInputSymbolsValidForLanguage(l:Language,inputS:InputSymbols)
+{
+    forall input:seq<string>::  input in l <==> 
+                                exists c:seq<string> :: isInputValid(input+c,inputS)
+}
+ghost predicate inputSymbolsForCKT (inputS:InputSymbols,l:Language)
+    requires isLanguageCKT(l)
+{
+    isInputSymbolsValidForLanguage(l,inputS)
+}
+ghost predicate AdditionalTapeSymbolsForCKT(inputS:InputSymbols,l:Language,addTapeS:AdditionalTapeSymbols)
+    requires isLanguageCKT(l)
+    requires isInputSymbolsValidForLanguage(l,inputS)
+{
+    isTapeSymbolsValid(inputS,addTapeS)
+}
+// lemma isCKTNP (l:Language)
+// requires isLanguageCKT(l)
+// ensures isLanguageNPTIME2(l)
+// {
+
+// }
