Certificate.dfy
@@ -1,0 +1,33 @@
+include "objects.dfy"
+include "turing_machine.dfy"
+type certificate=seq<string>
+ predicate isCertificateCorrectForm (k:certificate)
+{
+    (|k|>0 && |k|%2==0) && (forall pos:nat:: pos<|k| ==> (if pos%2==1 then 
+    (k[pos]!="TRUE" && k[pos]!="FALSE") 
+    else (k[pos]=="TRUE" || k[pos]=="FALSE"))) 
+}
+ function findValue(k:certificate,v:string) : Option<bool>
+    requires isCertificateCorrectForm(k)
+    requires v!="TRUE" && v!="FALSE"
+ {
+    findValue'(k,v,1)
+ }
+ function findValue'(k:certificate,v:string,pos:nat): Option<bool>
+    requires 0<pos<=|k|
+    requires isCertificateCorrectForm(k)
+    requires v!="TRUE" && v!="FALSE"
+    decreases |k|-pos
+
+ {
+    if pos==|k| then 
+        None
+    else
+        if k[pos]==v then
+            if k[pos-1]=="TRUE" then 
+                Some(true)
+            else
+                Some(false)
+        else
+            findValue'(k,v,pos+1)
+ }
