Circuit.dfy
@@ -1,0 +1,168 @@
+include "objects.dfy"
+include "Certificate.dfy"
+predicate isCircuitCellAPoz (e:circuitCell)
+{
+     match e
+        case POZ(nr) => true
+        case _ => false 
+}
+predicate isCircuitCellAVariable(e:circuitCell)
+{
+    match e 
+        case VARIABLE(_) => true
+        case _ => false
+}
+predicate isAGoodPoz (e:circuitCell,poz:nat)
+    requires isCircuitCellAPoz(e)
+{
+    match e
+        case POZ(nr) => (
+            0<=nr<=poz-1)
+}
+predicate isAGoodVariableCircuit(e:circuitCell)
+    requires isCircuitCellAVariable(e)
+{
+    match e 
+        case VARIABLE(x) => !isStringAValidNumber(x) && !(x in ReservedWords)
+}
+predicate isCircuitGood(c:circuit)
+{
+    forall poz:nat::poz<|c| ==> isCircuitGood'(c[poz],poz)
+}
+predicate isCircuitGood'(c:circuitCell,poz:nat)
+
+{
+    if isCircuitCellAPoz(c) then
+        isAGoodPoz(c,poz)
+    else
+        if isCircuitCellAVariable(c) then 
+            isAGoodVariableCircuit(c)
+        else true 
+}
+predicate isCircuitValid (c:circuit)
+{
+    forall pos:nat :: 0<=pos<|c| ==> isCircuitValid'(c,pos)
+}
+predicate isCircuitValid'(c:circuit, pos:nat)
+    requires pos<|c|
+{
+    match c[pos]
+            case AND => 2<pos<|c| && isCircuitCellAPoz(c[pos-1]) && isCircuitCellAPoz(c[pos-2])
+            case OR => 2<pos<|c|  && isCircuitCellAPoz(c[pos-1]) && isCircuitCellAPoz(c[pos-2])
+            case NOT => 1<pos<|c| && isCircuitCellAPoz(c[pos-1]) 
+            case VARIABLE (x) => isAGoodVariableCircuit(c[pos])
+            case POZ(nr) => isAGoodPoz(c[pos],pos) && !isCircuitCellAPoz(c[nr])
+}
+// predicate isThatPOZValid(c:circuit,pos:nat)
+//     requires pos<|c|
+// {
+//     match c[pos]
+//          case POZ(nr) =>  pos>0 && 0<nr<pos-1 && pos-nr-1>=0 && !isCircuitCellAPoz(c[nr])
+//          case _=>true
+// }
+
+predicate isCertificateValid (c:circuit,k:certificate)
+    requires isCertificateCorrectForm(k)
+    requires isCircuitValid(c)
+{
+     forall pos:nat:: pos<|c| ==> match c[pos]
+                                    case VARIABLE(x) => 
+                                    assert isCircuitValid'(c,pos);
+                                    assert !(x in ReservedWords);
+                                    findValue(k,x)!=None
+                                    case _ => true
+ }
+ lemma Lemma_ValidCircuitExtension(c: circuit, ext: seq<circuitCell>)
+    requires isCircuitValid(c)
+    requires forall k :: |c| <= k <|c|+ |ext| ==> isCircuitValid'(c + ext, k)
+    ensures isCircuitValid(c + ext)
+{
+    var combined := c + ext;
+
+    assert forall i :: 0 <= i < |c| ==> combined[i] == c[i];
+    assert forall i :: 0 <= i < |c| ==> isCircuitValid'(c, i);
+    assert forall i :: 0 <= i < |c| && isCircuitValid'(c,i)==> isCircuitValid'(combined, i);
+    assert isCircuitValid(combined);
+}
+ predicate variableHasValue(c:circuit,k:certificate,pos:nat)
+    requires pos<|c|
+ {
+    match c[pos] 
+                 case VARIABLE(x) => exists poz:nat :: (1<poz<|k| && (
+                     k[poz]==x && (k[poz-1]=="TRUE" && k[poz-1]=="FALSE"))) 
+                 case _ => true
+ }
+function getValueFromCertificate (v:string,k:certificate):Option<bool>
+     requires v!="FALSE" && v!="TRUE"
+     requires isCertificateCorrectForm (k)
+
+{
+    getValueFromCertificate'(v,k,0)
+}
+function getValueFromCertificate'(v:string,k:certificate,pos:nat):Option<bool>
+    requires pos<=|k|
+    requires v!="FALSE" && v!="TRUE"
+    decreases |k|-pos
+    ensures getValueFromCertificate'(v,k,pos)!=None <==>exists poz:nat :: (0<poz<|k| && (
+                    k[poz]==v && (k[poz-1]=="TRUE" || k[poz-1]=="FALSE")))
+    requires forall poz:nat ::poz<pos ==> k[poz]!=v
+    ensures forall poz:nat ::poz<pos ==>  k[poz]!=v
+    requires isCertificateCorrectForm(k)
+
+{
+    if pos==|k| then None
+    else
+        if k[pos]==v then(
+            assert  v!="FALSE" && v!="TRUE";
+            assert k[pos]!="TRUE" && k[pos]!="FALSE";
+            assert k[pos-1]=="TRUE" || k[pos-1]=="FALSE";
+            if k[pos-1]=="TRUE" then 
+                Some(true)
+            else
+                Some(false)
+            )
+        else
+            getValueFromCertificate'(v,k,pos+1)
+}
+predicate solveCircuit(c:circuit,k:certificate)
+    requires isCircuitValid(c)
+    requires isCertificateCorrectForm(k)
+    requires isCertificateValid(c,k)
+    requires |c|>=1
+{
+    solveCircuit'(c,k,|c|-1)
+}
+predicate solveCircuit'(c:circuit,k:certificate,pos:nat)
+    requires isCircuitValid(c)
+    requires |k|>=1 && |k|%2==0
+    requires isCertificateCorrectForm(k)
+    requires isCertificateValid(c,k)
+    requires |c|>=1
+    requires pos<|c|
+    decreases pos
+{
+
+    match c[pos]
+        case AND =>  
+            assert  isCircuitValid'(c, pos);
+            solveCircuit'(c,k,pos-1) && solveCircuit'(c,k,pos-2)
+        case OR  =>
+            assert  isCircuitValid'(c, pos);
+            solveCircuit'(c,k,pos-1) || solveCircuit'(c,k,pos-2)
+        case NOT  =>
+            assert  isCircuitValid'(c, pos);        
+        !solveCircuit'(c,k,pos-1)
+        case VARIABLE (x) =>( assert isCircuitValid'(c,pos);     
+            match findValue(k,x)
+                                        case Some(st) => st
+                                        case None => false )
+        case POZ(nr)=>
+            assert  isCircuitValid'(c, pos);
+            solveCircuit'(c,k,nr)
+}
+
+ghost predicate checkSatisfaction(c:circuit)
+    requires isCircuitValid(c)
+{
+    exists k:certificate :: isCertificateCorrectForm(k) && isCertificateValid(c,k) && |c|>=1 && solveCircuit(c,k)
+}
