objects.dfy
@@ -1,0 +1,41 @@
+datatype circuitCell = AND | OR | NOT | VARIABLE(x:string) | POZ(i:nat)
+type circuit=seq<circuitCell>
+type stringNat = s: string |
+    |s| > 0 && (|s| > 1 ==> s[0] != '0') &&
+    forall i | 0 <= i < |s| :: s[i] in "0123456789"
+    witness "1"
+const ReservedWords:=["AND","OR","NOT","TRUE","FALSE","CERTIFICATE"]
+predicate isStringAValidNumber (s:string)
+{
+    |s| > 0 && (|s| > 1 ==> s[0] != '0') &&
+    forall i | 0 <= i < |s| :: s[i] in "0123456789"
+}
+  function natToString(n: nat): string
+    ensures isStringAValidNumber(natToString(n))
+   {
+    match n
+    case 0 => "0" case 1 => "1" case 2 => "2" case 3 => "3" case 4 => "4"
+    case 5 => "5" case 6 => "6" case 7 => "7" case 8 => "8" case 9 => "9"
+    case _ => natToString(n / 10) + natToString(n % 10)
+  }
+
+  function stringToNat(s: string): nat
+    decreases |s|
+    requires isStringAValidNumber(s)
+  {
+    if |s| == 1 then
+      match s[0]
+      case '0' => 0 case '1' => 1 case '2' => 2 case '3' => 3 case '4' => 4
+      case '5' => 5 case '6' => 6 case '7' => 7 case '8' => 8 case '9' => 9
+    else
+      stringToNat(s[..|s|-1])*10 + stringToNat(s[|s|-1..|s|])
+  }
+  lemma natToStringThenStringToNatIdem(n: nat)
+    ensures stringToNat(natToString(n)) == n
+  { 
+  }
+  lemma stringToNatThenNatToStringIdem(n: string)
+    requires isStringAValidNumber(n)
+    ensures natToString(stringToNat(n)) == n
+  { 
+  }
